src/xor/xor.lean
@@ -28,6 +28,16 @@ open clause
 open cnf
 open explode
 
+-- The conversion of the XOR gate to a clause is a nice way of sweeping
+-- uner the rug that the two definitions are actually identical
+-- TODO canonical way of saying we want the nil/empty clause?
+def to_clause (g : xor_gate) : clause :=
+  g.foldr (λ l c, l :: c) []
+
+-- Kinda cheesy
+lemma gate_eq_clause (g : xor_gate) : g = g.to_clause :=
+by simp [to_clause]
+
 /- Evaluates the XOR gate under an assignment -/
 def eval (α : assignment) (g : xor_gate) : bool :=
   g.foldr (λ l b, b ⊕ l.eval α) ff
@@ -51,7 +61,7 @@ def eval_rec (α : assignment) : xor_gate → bool
 | (l :: ls) := l.eval α ⊕ eval_rec ls
 
 /- To use the recursive definition, we need to prove that the two functions are equivalent -/
-theorem eval_and_eval_rec_equiv {α : assignment} {g : xor_gate} : eval α g = eval_rec α g :=
+theorem eval_and_eval_rec_equiv (α : assignment) (g : xor_gate) : eval α g = eval_rec α g :=
 begin
   induction g with l ls ih,
   { simp [eval_rec, eval] },
@@ -59,13 +69,26 @@ begin
 end
 
 /- The XOR gate evaluates to true if an odd number of literals evaluates to true -/
-theorem xor_odd_eval_tt {α : assignment} {g : xor_gate} : g.eval α = nat.bodd (g.countp (λ l, l.eval α = tt)) :=
+theorem xor_odd_eval_tt (α : assignment) (g : xor_gate) : g.eval α = nat.bodd (g.countp (λ l, l.eval α = tt)) :=
 begin
   induction g with l ls ih,
   split; { simp [eval] },
   by_cases (l.eval α = tt),
   { simp [h, ih, eval_cons] },
   { simp at h, simp [h, ih, eval_cons] }
+end
+
+theorem xor_odd_eval_tt2 (α : assignment) (g : xor_gate) : g.eval α = nat.bodd (g.to_clause.count_tt α) :=
+begin
+  induction g with l ls ih,
+  { simp [to_clause] },
+  {
+    by_cases (l.eval α = tt),
+    { rw ← gate_eq_clause ls at ih,
+      simp [to_clause, eval_cons, count_tt_cons, bool.to_nat, h, ih] },
+    { simp at h,
+      rw ← gate_eq_clause ls at ih,
+      simp [to_clause, eval_cons, count_tt_cons, bool.to_nat, h, ih] } }
 end
 
 -- Let's start easier: turning a list of natural numbers into a cnf form
@@ -75,6 +98,20 @@ def nat_to_xor_cnf : list nat → cnf
 | []        := [[]]
 | (n :: ns) := (explode ns).map (λ c, cond (nat.bodd c.count_neg = ff) ((Pos n) :: c) ((Neg n) :: c))
 
+-- Riskier, but what else can you do?
+theorem mem_explode_of_mem_nat_to_xor :
+  ∀ {ns : list nat}, ∀ {c : clause}, c ∈ nat_to_xor_cnf ns → c ∈ explode ns
+| []        := by simp [nat_to_xor_cnf]
+| (n :: ns) := begin
+  simp [nat_to_xor_cnf, mem_map, mem_append],
+  intros c hc,
+  by_cases c.count_neg.bodd = tt,
+  { simp [h], have : (Pos n).var = n, simp [var],
+    exact mem_explode_cons_of_lit c hc this },
+  { simp [bool_eq_false h], have : (Neg n).var = n, simp [var],
+    exact mem_explode_cons_of_lit c hc this }
+end
+
 theorem nat_to_xor_cnf_length {ns : list nat} : ns ≠ [] → length (nat_to_xor_cnf ns) = 2^(length ns - 1) :=
 begin
   cases classical.em (ns = nil); intro hns,
@@ -83,6 +120,37 @@ begin
     simp only [nat_to_xor_cnf, length_map, length_cons, length_explode, nat.succ_sub_one] }
 end
 
+theorem exists_mem_nat_to_xor_of_ne_nil {ns : list nat} : ns ≠ [] → ∃ (c : clause), c ∈ nat_to_xor_cnf ns :=
+begin
+  induction ns with m ms ih,
+  { contradiction },
+  { intro _,
+    by_cases hms : ms = [],
+    { use (Pos m) :: [],
+      simp [hms, nat_to_xor_cnf] },
+    { 
+      rcases ih hms with ⟨c, hc⟩,
+      by_cases nat.bodd c.count_neg = ff,
+      { use (Pos m :: c),
+        simp [nat_to_xor_cnf],
+        use c,
+        simp [mem_explode_of_mem_nat_to_xor hc, h] },
+      { use (Neg m :: c),
+        simp [nat_to_xor_cnf],
+        use c,
+        simp [mem_explode_of_mem_nat_to_xor hc, h] } } }
+end
+
+theorem map_var_eq_of_mem_nat_to_xor : ∀ {ns : list nat}, ∀ {c : clause}, c ∈ nat_to_xor_cnf ns → c.map var = ns
+| []        := by { simp [nat_to_xor_cnf] }
+| (n :: ns) := begin
+  simp [nat_to_xor_cnf],
+  intros c hc,
+  by_cases c.count_neg.bodd = ff;
+  { simp [h, var, map_var_eq_of_mem_explode hc] }
+end
+
+-- Can be shortened to one or two lines given aboce theorem, as sim. is weaker
 theorem map_var_sim_of_mem_nat_to_xor : ∀ (ns : list nat), ∀ (c : clause), c ∈ nat_to_xor_cnf ns → c.map var ~ ns
 | []        := by { simp [nat_to_xor_cnf] }
 | (n :: ns) := begin
@@ -97,19 +165,7 @@ theorem exists_mem_explode_sim_of_mem_nat_to_xor {ns : list nat} :
   ∀ (c : clause), c ∈ nat_to_xor_cnf ns → ∃ cl ∈ explode ns, c ~ cl :=
 assume c h, mem_explode_sim_of_map_var_sim c (map_var_sim_of_mem_nat_to_xor ns c h)
 
--- Riskier, but what else can you do?
-theorem exists_mem_explode_of_mem_nat_to_xor :
-  ∀ (ns : list nat), ∀ (c : clause), c ∈ nat_to_xor_cnf ns → c ∈ explode ns
-| []        := by simp [nat_to_xor_cnf]
-| (n :: ns) := begin
-  simp [nat_to_xor_cnf, mem_map, mem_append],
-  intros c hc,
-  by_cases c.count_neg.bodd = tt,
-  { simp [h], have : (Pos n).var = n, simp [var],
-    exact mem_explode_cons_of_lit c hc this },
-  { simp [bool_eq_false h], have : (Neg n).var = n, simp [var],
-    exact mem_explode_cons_of_lit c hc this }
-end
+
 
 -- Technically not a proof by induction, fix later?
 theorem nat_to_xor_cnf_contains_all_even_negated_clauses {ns : list nat} :
@@ -125,54 +181,98 @@ begin
     simp [hcount, mem_explode_of_map_var_eq hls] } }
 end
 
--- TODO cleanup
-theorem nat_to_xor_cnf_contains_no_even_negated_clauses {ns : list nat} (hns: ns ≠ []) :
-  ∀ {c : clause}, c.map var = ns → (nat.bodd c.count_neg = tt) → c ∉ nat_to_xor_cnf ns :=
+-- Not really induction, switch later
+theorem even_negation_of_mem_nat_to_xor {ns : list nat} :
+  ∀ {c : clause}, c.map var = ns → c ∈ nat_to_xor_cnf ns → nat.bodd c.count_neg = ff :=
 begin
   induction ns with m ms ih,
-  { contradiction },
-  {
-    intros c hc,
-    rcases exists_cons_of_map_cons hc with ⟨l, ls, rfl, hl, hls⟩,
-    rcases pos_or_neg_of_var_eq_nat hl with rfl | rfl,
-    { simp [count_neg_cons, is_neg, bool.to_nat, nat_to_xor_cnf],
-      intros hcount x hx,
-      by_cases (count_neg x).bodd = tt,
-      { simp [h], intro h2,
-        exact absurd (head_eq_of_cons_eq h2) ne_pos_neg_of_nat.symm },
-      { simp [bool_eq_false h], -- Lots of fooling around with ¬ and ff, clean up
-        intro h2, have h2 := tail_eq_of_cons_eq h2,
-        rw h2 at h,
-        rw hcount at h,
-        exact absurd (refl tt) h } },
-    { simp [count_neg_cons, is_neg, bool.to_nat, nat_to_xor_cnf],
-      intros hcount x hx,
-      by_cases (count_neg x).bodd = tt,
-      { simp [h], intro h2,
-        have h2 := tail_eq_of_cons_eq h2,
-        rw h2 at h,
-        exact bool_iff_false.mpr hcount h },
-      { simp [bool_eq_false h], intro h2,
-        exact absurd (head_eq_of_cons_eq h2) ne_pos_neg_of_nat } } }
+  { simp },
+  intros c hc hxor,
+  simp [nat_to_xor_cnf] at hxor,
+  rcases hxor with ⟨a, ha, hacons⟩,
+  rcases exists_cons_of_map_cons hc with ⟨l, ls, rfl, hl, hls⟩,
+  by_cases a.count_neg.bodd = ff,
+  { simp [h] at hacons,
+    simp [← hacons, count_neg_cons, is_neg, bool.to_nat, h] },
+  { simp [h] at hacons,
+    simp at h,
+    simp [← hacons, count_neg_cons, is_neg, bool.to_nat, h] }
+end
+
+theorem even_negation_iff_mem_nat_to_xor {ns : list nat} {c : clause} (hc : c.map var = ns) :
+  c ∈ nat_to_xor_cnf ns ↔ nat.bodd c.count_neg = ff :=
+⟨even_negation_of_mem_nat_to_xor hc, nat_to_xor_cnf_contains_all_even_negated_clauses hc⟩
+
+theorem nat_to_xor_cnf_contains_no_odd_negated_clauses {ns : list nat} :
+  ∀ {c : clause}, c.map var = ns → (nat.bodd c.count_neg = tt) → c ∉ nat_to_xor_cnf ns :=
+begin
+  intros c hc hcount,
+  by_cases c ∈ nat_to_xor_cnf ns, -- This is a little cheesy, but I want to show contradiction
+  { have red := even_negation_of_mem_nat_to_xor hc h,
+    rw hcount at red,
+    exact absurd red (ne.symm ff_eq_tt_eq_false) },
+  { exact h }
+end
+
+-- TODO move the c.map var assumption into the ns list nat portion since the above need it too
+theorem odd_negation_of_not_mem_nat_to_xor {ns : list nat} :
+  ∀ {c : clause}, c.map var = ns → c ∉ nat_to_xor_cnf ns → nat.bodd c.count_neg = tt :=
+begin
+  intros c hc,
+  contrapose,
+  simp,
+  intro hcount,
+  exact nat_to_xor_cnf_contains_all_even_negated_clauses hc hcount
+end
+
+theorem odd_negation_iff_not_mem_nat_to_xor {ns : list nat} {c : clause} (hc : c.map var = ns) :
+  c ∉ nat_to_xor_cnf ns ↔ nat.bodd c.count_neg = tt :=
+⟨odd_negation_of_not_mem_nat_to_xor hc, nat_to_xor_cnf_contains_no_odd_negated_clauses hc⟩
+
+-- TODO clean up, e.g. by apply
+theorem true_forward {α : assignment} : ∀ {ns : list nat} (hnodup: ns.nodup), eval α (ns.map Pos) = tt → cnf.eval α (nat_to_xor_cnf ns) = tt
+| []        := by simp
+| (n :: ns) := begin
+  intros hnsnodup h,
+  have red := xor_odd_eval_tt2 α (map Pos (n :: ns)),
+  rw h at red,
+  rw ← gate_eq_clause (map Pos (n :: ns)) at red,
+  have : ∀ (c : clause), c ∈ nat_to_xor_cnf (n :: ns) → clause.eval α c = tt,
+  { intros c hc,
+    have mapvareq : map var c = (n :: ns), from map_var_eq_of_mem_nat_to_xor hc,
+    have : nat.bodd c.count_neg = ff, from even_negation_of_mem_nat_to_xor mapvareq hc,
+    have neq : nat.bodd (count_tt α (map Pos (n :: ns))) ≠ nat.bodd c.count_neg,
+      from neq_of_ff_of_tt (eq.symm red) this,
+    exact eval_tt_of_opposite_parity (cons_ne_nil n ns) hnsnodup mapvareq neq },
+  exact eval_tt_iff_clauses_tt.mpr this
+end
+
+-- TODO clean up
+theorem false_forward {α : assignment} : ∀ {ns : list nat} (hnodup : ns.nodup), eval α (ns.map Pos) = ff → cnf.eval α (nat_to_xor_cnf ns) = ff
+| []        := by simp [nat_to_xor_cnf]
+| (n :: ns) := begin
+  intros hnsnodup h,
+  have red := xor_odd_eval_tt2 α (map Pos (n :: ns)),
+  rw h at red,
+  rw ← gate_eq_clause (map Pos (n :: ns)) at red,
+  apply eval_ff_iff_exists_clause_ff.mpr,
+  have : count_tt α (map Pos (n :: ns)) = count_neg (falsify α (n :: ns)), 
+    from count_tt_pos_eq_count_neg_falsify α (n :: ns),
+  have : nat.bodd (count_tt α (map Pos (n :: ns))) = nat.bodd (count_neg (falsify α (n :: ns))), 
+    from congr_arg nat.bodd this,
+  rw ← red at this,
+  have mapvareq := nat_to_xor_cnf_contains_all_even_negated_clauses (map_var_falsify_eq_list α (n :: ns)) this.symm,
+  use (falsify α (n :: ns)),
+  simp [mapvareq, eval_ff_of_falsify α (n :: ns)]
 end
 
 -- We prove that the naive encoding is equivalent to an XOR gate of all positive literals
-theorem nat_to_xor_cnf_correct {α : assignment} : ∀ (ns : list nat), cnf.eval α (nat_to_xor_cnf ns) = eval α (ns.map Pos)
-| []        := by simp [nat_to_xor_cnf]
-| (n :: ns) := begin
-  --simp [nat_to_xor_cnf, map_cons, eval_cons],
-  by_cases ((map Pos (n :: ns)).countp (λ l, literal.eval α l = tt)).bodd = tt,
-  { --  We are in the odd case, meaning that we should satisfy
-    have : eval α (map Pos (n :: ns)) = ((map Pos (n :: ns)).countp (λ l, literal.eval α l = tt)).bodd, from xor_odd_eval_tt,
-    rw this.symm at h,
-    rw h,
-    simp [nat_to_xor_cnf],
-    sorry,
-
-
-  }
-  sorry,
-  sorry,
+theorem nat_to_xor_cnf_correct (α : assignment) {ns : list nat} (hns : ns.nodup) : 
+  cnf.eval α (nat_to_xor_cnf ns) = eval α (ns.map Pos) :=
+begin
+  rcases bool_by_cases (eval α (map Pos ns)) with h | h,
+  { simp [h, true_forward hns] },
+  { simp [h, false_forward hns] }
 end
 
 end xor_gate
