src/basic.lean
@@ -10,6 +10,8 @@
 import data.bool
 import data.list.basic
 
+open list
+
 -- Define shorthand for XOR
 notation a ⊕ b := bxor a b
 --notation a ∨ b := bor a b
@@ -36,13 +38,38 @@ theorem bxor_disjunctive : ∀ (a b : bool), bxor a b = (!a && b) || (a && !b)
 | ff tt := dec_trivial
 | ff ff := dec_trivial
 
+theorem neq_of_ff_of_tt {a b : bool} : a = tt → b = ff → a ≠ b :=
+begin
+  intros ha hb, simp [ha, hb]
+end
+
+theorem bool_by_cases : ∀ (b : bool), b = tt ∨ b = ff
+| tt := by { left, refl }
+| ff := by { right, refl }
+
 -- Some facts about map that help
+theorem exists_of_map_singleton {α β : Type} {f : α → β} {b : β} :
+  ∀ {l : list α}, map f l = [b] → ∃ a, [a] = l ∧ f a = b
+| []        := by { contradiction }
+| [x]       := by { simp [map_cons] }
+| (x :: y :: ys) := by { simp }
+
 theorem exists_cons_of_map_cons {α β : Type} {f : α → β} {b : β} {bs : list β} :
-  ∀ {l : list α}, list.map f l = b :: bs → ∃ h L, l = h :: L ∧ f h = b ∧ list.map f L = bs
-| [] := by { contradiction }
+  ∀ {l : list α}, map f l = b :: bs → ∃ h L, l = h :: L ∧ f h = b ∧ map f L = bs
+| []        := by { contradiction }
 | (x :: xs) := begin 
-  simp [list.map_cons],
-  intros hx hxs, split,
-  { use x, exact hx},
-  { use xs, exact hxs}
+  simp [map_cons],
+  intros hx hxs,
+  use x, use xs, simp [hx, hxs]
+end
+
+-- Or facts about filter
+theorem length_filter {α : Type} {p : α → Prop} [decidable_pred p] {l : list α} : 
+  length (filter p l) ≤ length l :=
+begin
+  induction l with x xs ih,
+  { simp },
+  { by_cases p x,
+    { simp [filter_cons_of_pos _ h, ih] },
+    { simp [filter_cons_of_neg _ h, ih, le_add_right] } }
 end
